finishing the 2 effects setup, no examples yet

pulse/ulib/experimental/Steel.Effects2.fst
@@ -66,15 +66,21 @@ type repr (a:Type) (pre:pre_t) (post:post_t a) (req:req_t pre) (ens:ens_t pre a 
 
 assume val sl_implies (p q:hprop u#1) : Type0
 
+assume val sl_implies_reflexive (p:hprop u#1)
+: Lemma (p `sl_implies` p)
+  [SMTPat (p `sl_implies` p)]
+
 assume val sl_implies_interp (p q:hprop u#1)
 : Lemma
   (requires p `sl_implies` q)
   (ensures forall (m:mem) (f:hprop). interp (p `star` f) m ==>  interp (q `star` f) m)
+  [SMTPat (p `sl_implies` q)]
 
 assume val sl_implies_interp_emp (p q:hprop u#1)
 : Lemma
   (requires p `sl_implies` q)
   (ensures forall (m:mem). interp p m ==>  interp q m)
+  [SMTPat (p `sl_implies` q)]
 
 assume val sl_implies_preserves_frame (p q:hprop u#1)
 : Lemma
@@ -83,6 +89,7 @@ assume val sl_implies_preserves_frame (p q:hprop u#1)
     forall (m1 m2:mem) (r:hprop).
       Sem.preserves_frame #state q r m1 m2 ==>
       Sem.preserves_frame #state p r m1 m2)
+  [SMTPat (p `sl_implies` q)]
 
 assume val sl_implies_preserves_frame_right (p q:hprop u#1)
 : Lemma
@@ -91,13 +98,14 @@ assume val sl_implies_preserves_frame_right (p q:hprop u#1)
     forall (m1 m2:mem) (r:hprop).
       Sem.preserves_frame #state r p m1 m2 ==>
       Sem.preserves_frame #state r q m1 m2)
+  [SMTPat (p `sl_implies` q)]
 
 
 unfold
 let return_req (p:hprop u#1) : req_t p = fun _ -> True
 
 unfold
-let return_ens (#a:Type) (x:a) (p:a -> hprop u#1) : ens_t (p x) a p = fun _ r _ -> r == x
+let return_ens (a:Type) (x:a) (p:a -> hprop u#1) : ens_t (p x) a p = fun _ r _ -> r == x
 
 (*
  * Return is parametric in post
@@ -106,35 +114,49 @@ let return_ens (#a:Type) (x:a) (p:a -> hprop u#1) : ens_t (p x) a p = fun _ r _ 
  *   (cf. return-scoping.txt)
  *)
 let return (a:Type) (x:a) (p:a -> hprop)
-: repr a (p x) p (return_req (p x)) (return_ens x p)
+: repr a (p x) p (return_req (p x)) (return_ens a x p)
 = fun _ -> x
 
+(*
+ * We allow weakening of post resource of f to pre resource of g
+ *)
 unfold
-let bind_req (#a:Type) (#pre_f:pre_t) (#post_f:post_t a)
-  (req_f:req_t pre_f) (ens_f:ens_t pre_f a post_f)
-  (req_g:(x:a -> req_t (post_f x)))
+let bind_req (a:Type)
+  (pre_f:pre_t) (post_f:post_t a)
+  (req_f:req_t pre_f) (ens_f:ens_t pre_f a post_f)  
+  (pre_g:a -> pre_t)
+  (req_g:(x:a -> req_t (pre_g x)))
+  (_:squash (forall (x:a). post_f x `sl_implies` pre_g x))
 : req_t pre_f
-= fun m0 -> req_f m0 /\ (forall (x:a) (m1:hmem (post_f x)). ens_f m0 x m1 ==> (req_g x) m1)
+= fun m0 ->
+  req_f m0 /\
+  (forall (x:a) (m1:hmem (post_f x)). ens_f m0 x m1 ==> (req_g x) m1)
 
 unfold
-let bind_ens (#a:Type) (#b:Type)
-  (#pre_f:pre_t) (#post_f:post_t a) (req_f:req_t pre_f) (ens_f:ens_t pre_f a post_f)
-  (#post_g:post_t b) (ens_g:(x:a -> ens_t (post_f x) b post_g))
+let bind_ens (a:Type) (b:Type)
+  (pre_f:pre_t) (post_f:post_t a)
+  (req_f:req_t pre_f) (ens_f:ens_t pre_f a post_f)  
+  (pre_g:a -> pre_t) (post_g:post_t b)
+  (ens_g:(x:a -> ens_t (pre_g x) b post_g))
+  (_:squash (forall (x:a). post_f x `sl_implies` pre_g x))
 : ens_t pre_f b post_g
 = fun m0 y m2 ->
-  req_f m0 /\ (exists (x:a) (m1:hmem (post_f x)). ens_f m0 x m1 /\ (ens_g x) m1 y m2)
+  req_f m0 /\
+  (exists (x:a) (m1:hmem (post_f x)). ens_f m0 x m1 /\ (ens_g x) m1 y m2)
 
-(*
- * This bind is a simple bind that enforces f post to be
- *   definitionally equal to g pre
- * This is just for effect definition
- * Later we define polymonadic binds that relax this and provide framing support
- *)
 let bind (a:Type) (b:Type)
-  (pre_f:pre_t) (post_f:post_t a) (req_f:req_t pre_f) (ens_f:ens_t pre_f a post_f)
-  (post_g:post_t b) (req_g:(x:a -> req_t (post_f x))) (ens_g:(x:a -> ens_t (post_f x) b (post_g)))
-  (f:repr a pre_f post_f req_f ens_f) (g:(x:a -> repr b (post_f x) post_g (req_g x) (ens_g x)))
-: repr b pre_f post_g (bind_req req_f ens_f req_g) (bind_ens req_f ens_f ens_g)
+  (pre_f:pre_t) (post_f:post_t a)
+  (req_f:req_t pre_f) (ens_f:ens_t pre_f a post_f)  
+  (pre_g:a -> pre_t) (post_g:post_t b)
+  (req_g:(x:a -> req_t (pre_g x))) (ens_g:(x:a -> ens_t (pre_g x) b post_g))
+  (p:squash (forall (x:a). post_f x `sl_implies` pre_g x))
+  (f:repr a pre_f post_f req_f ens_f)
+  (g:(x:a -> repr b (pre_g x) post_g (req_g x) (ens_g x)))
+: repr b
+    pre_f
+    post_g
+    (bind_req a pre_f post_f req_f ens_f pre_g req_g p)
+    (bind_ens a b pre_f post_f req_f ens_f pre_g post_g ens_g p)
 = fun _ ->
   let x = f () in
   (g x) ()
@@ -144,37 +166,59 @@ let bind (a:Type) (b:Type)
  * TODO: don't use polymonadic binds for lift anymore
  *)
 
-
 (*
  * f <: g
  *)
+
 unfold
-let subcomp_pre (#a:Type) (#pre_f:pre_t) (#post_f:post_t a)
-  (req_f:req_t pre_f) (ens_f:ens_t pre_f a post_f)
-  (#pre_g:pre_t) (#post_g:post_t a)
-  (req_g:req_t pre_g) (ens_g:ens_t pre_g a post_g)
+let subcomp_pre (a:Type)
+  (pre_f:pre_t) (post_f:post_t a) (req_f:req_t pre_f) (ens_f:ens_t pre_f a post_f)
+  (pre_g:pre_t) (post_g:post_t a) (req_g:req_t pre_g) (ens_g:ens_t pre_g a post_g)
   (_:squash (pre_g `sl_implies` pre_f))
   (_:squash (forall (x:a). post_f x `sl_implies` post_g x))
 : pure_pre
-= (forall (m0:hmem pre_g). req_g m0 ==> req_f m0)
-
-
+= (forall (m0:hmem pre_g). req_g m0 ==> req_f m0) /\
+  (forall (m0:hmem pre_g) (x:a) (m1:hmem (post_f x)). ens_f m0 x m1 ==> ens_g m0 x m1)
 
 let subcomp (a:Type)
-  (pre_f:pre_t) (post_f:post_t a) (f:repr a pre_f post_f)
-: repr a pre_f post_f
+  (pre_f:pre_t) (post_f:post_t a) (req_f:req_t pre_f) (ens_f:ens_t pre_f a post_f)
+  (pre_g:pre_t) (post_g:post_t a) (req_g:req_t pre_g) (ens_g:ens_t pre_g a post_g)
+  (p1:squash (pre_g `sl_implies` pre_f))
+  (p2:squash (forall (x:a). post_f x `sl_implies` post_g x))
+  (f:repr a pre_f post_f req_f ens_f)
+: Pure (repr a pre_g post_g req_g ens_g)
+  (requires subcomp_pre a pre_f post_f req_f ens_f pre_g post_g req_g ens_g p1 p2)
+  (ensures fun _ -> True)
 = f
-  
-let if_then_else (a:Type)
-  (pre:pre_t) (post:post_t a)
-  (f:repr a pre post) (g:repr a pre post)
+
+unfold
+let if_then_else_req (pre:pre_t)
+  (req_then:req_t pre) (req_else:req_t pre)
+  (p:Type0)
+: req_t pre
+= fun h -> (p ==> req_then h) /\ ((~ p) ==> req_else h)
+
+unfold
+let if_then_else_ens (a:Type) (pre:pre_t) (post:post_t a)
+  (ens_then:ens_t pre a post) (ens_else:ens_t pre a post)
+  (p:Type0)
+: ens_t pre a post
+= fun h0 x h1 -> (p ==> ens_then h0 x h1) /\ ((~ p) ==> ens_else h0 x h1)
+
+let if_then_else (a:Type) (pre:pre_t) (post:post_t a)
+  (req_then:req_t pre) (ens_then:ens_t pre a post)
+  (req_else:req_t pre) (ens_else:ens_t pre a post)
+  (f:repr a pre post req_then ens_then)
+  (g:repr a pre post req_else ens_else)
   (p:Type0)
 : Type
 = repr a pre post
+    (if_then_else_req pre req_then req_else p)
+    (if_then_else_ens a pre post ens_then ens_else p)
 
 reifiable reflectable
 layered_effect {
-  SteelF: a:Type -> pre_t -> post_t a -> Effect
+  SteelF: a:Type -> pre:pre_t -> post:post_t a -> req_t pre -> ens_t pre a post -> Effect
   with repr = repr;
        return = return;
        bind = bind;
@@ -184,92 +228,217 @@ layered_effect {
 
 new_effect Steel = SteelF
 
-let frame_aux (#a:Type) (#pre:pre_t) (#post:post_t a)
-  (f:repr a pre post) (frame:hprop)
-: repr a (pre `star` frame) (fun x -> post x `star` frame)
+(*
+ * Keeping f_frame aside for now
+ *)
+let frame_aux (#a:Type) (#pre:pre_t) (#post:post_t a) (#req:req_t pre) (#ens:ens_t pre a post)
+  ($f:repr a pre post req ens) (frame:hprop)
+: repr a (pre `star` frame) (fun x -> post x `star` frame) req ens
 = fun _ ->
   Sem.run #state #_ #_ #_ #_ #_ (Sem.Frame (Sem.Act f) frame (fun _ -> True))
 
-let bind_steel_steel (a:Type) (b:Type)
-  (pre_f:pre_t) (post_f:post_t a) (pre_g:a -> pre_t) (post_g:post_t b)
+
+(*
+ * Onto polymonadic binds
+ *)
+
+(*
+ * First the bind between two unframed computations
+ *
+ * Add a frame to each
+ *)
+
+unfold
+let bind_steel_steel_req (a:Type)
+  (pre_f:pre_t) (post_f:post_t a)
+  (req_f:req_t pre_f) (ens_f:ens_t pre_f a post_f)  
+  (pre_g:a -> pre_t)
+  (req_g:(x:a -> req_t (pre_g x)))
   (frame_f:hprop) (frame_g:hprop)
   (_:squash (forall (x:a). (post_f x `star` frame_f) `sl_implies` (pre_g x `star` frame_g)))
-  (f:repr a pre_f post_f) (g:(x:a -> repr b (pre_g x) post_g))
-: repr b (pre_f `star` frame_f) (fun z -> post_g z `star` frame_g)
+: req_t (pre_f `star` frame_f)
+= fun m0 ->
+  req_f m0 /\
+  (forall (x:a) (m1:hmem (post_f x `star` frame_f)). ens_f m0 x m1 ==> (req_g x) m1)
+
+unfold
+let bind_steel_steel_ens (a:Type) (b:Type)
+  (pre_f:pre_t) (post_f:post_t a)
+  (req_f:req_t pre_f) (ens_f:ens_t pre_f a post_f)  
+  (pre_g:a -> pre_t) (post_g:post_t b)
+  (ens_g:(x:a -> ens_t (pre_g x) b post_g))
+  (frame_f:hprop) (frame_g:hprop)
+  (_:squash (forall (x:a). (post_f x `star` frame_f) `sl_implies` (pre_g x `star` frame_g)))
+: ens_t (pre_f `star` frame_f) b (fun y -> post_g y `star` frame_g)
+= fun m0 y m2 ->
+  req_f m0 /\
+  (exists (x:a) (m1:hmem (post_f x `star` frame_f)). ens_f m0 x m1 /\ (ens_g x) m1 y m2)
+
+let bind_steel_steel (a:Type) (b:Type)
+  (pre_f:pre_t) (post_f:post_t a)
+  (req_f:req_t pre_f) (ens_f:ens_t pre_f a post_f)  
+  (pre_g:a -> pre_t) (post_g:post_t b)
+  (req_g:(x:a -> req_t (pre_g x))) (ens_g:(x:a -> ens_t (pre_g x) b post_g))
+  (frame_f:hprop) (frame_g:hprop)
+  (p:squash (forall (x:a). (post_f x `star` frame_f) `sl_implies` (pre_g x `star` frame_g)))
+  (f:repr a pre_f post_f req_f ens_f)
+  (g:(x:a -> repr b (pre_g x) post_g (req_g x) (ens_g x)))
+: repr b
+    (pre_f `star` frame_f)
+    (fun y -> post_g y `star` frame_g)
+    (bind_steel_steel_req a pre_f post_f req_f ens_f pre_g req_g frame_f frame_g p)
+    (bind_steel_steel_ens a b pre_f post_f req_f ens_f pre_g post_g ens_g frame_f frame_g p)
 = fun _ ->
   let x = frame_aux f frame_f () in
-
-  sl_implies_interp (post_f x `star` frame_f) (pre_g x `star` frame_g);
-  sl_implies_preserves_frame (post_f x `star` frame_f) (pre_g x `star` frame_g);
-  
   frame_aux (g x) frame_g ()
+
+
+(*
+ * Note that the output is a framed computation, hence SteelF
+ *)
 
 polymonadic_bind (Steel, Steel) |> SteelF = bind_steel_steel
 
 
-let bind_steel_steelf (a:Type) (b:Type)
-  (pre_f:pre_t) (post_f:post_t a) (pre_g:a -> pre_t) (post_g:post_t b)
+(*
+ * Steel, SteelF: frame the first computation
+ *)
+
+unfold
+let bind_steel_steelf_req (a:Type)
+  (pre_f:pre_t) (post_f:post_t a)
+  (req_f:req_t pre_f) (ens_f:ens_t pre_f a post_f)  
+  (pre_g:a -> pre_t)
+  (req_g:(x:a -> req_t (pre_g x)))
   (frame_f:hprop)
-  (_:squash (forall x. (post_f x `star` frame_f) `sl_implies` pre_g x))
-  (f:repr a pre_f post_f) (g:(x:a -> repr b (pre_g x) post_g))
-: repr b (pre_f `star` frame_f) post_g
+  (_:squash (forall (x:a). (post_f x `star` frame_f) `sl_implies` pre_g x))
+: req_t (pre_f `star` frame_f)
+= fun m0 ->
+  req_f m0 /\
+  (forall (x:a) (m1:hmem (post_f x `star` frame_f)). ens_f m0 x m1 ==> (req_g x) m1)
+
+unfold
+let bind_steel_steelf_ens (a:Type) (b:Type)
+  (pre_f:pre_t) (post_f:post_t a)
+  (req_f:req_t pre_f) (ens_f:ens_t pre_f a post_f)  
+  (pre_g:a -> pre_t) (post_g:post_t b)
+  (ens_g:(x:a -> ens_t (pre_g x) b post_g))
+  (frame_f:hprop)
+  (_:squash (forall (x:a). (post_f x `star` frame_f) `sl_implies` pre_g x))
+: ens_t (pre_f `star` frame_f) b post_g
+= fun m0 y m2 ->
+  req_f m0 /\
+  (exists (x:a) (m1:hmem (post_f x `star` frame_f)). ens_f m0 x m1 /\ (ens_g x) m1 y m2)
+
+let bind_steel_steelf (a:Type) (b:Type)
+  (pre_f:pre_t) (post_f:post_t a)
+  (req_f:req_t pre_f) (ens_f:ens_t pre_f a post_f)  
+  (pre_g:a -> pre_t) (post_g:post_t b)
+  (req_g:(x:a -> req_t (pre_g x))) (ens_g:(x:a -> ens_t (pre_g x) b post_g))
+  (frame_f:hprop)
+  (p:squash (forall (x:a). (post_f x `star` frame_f) `sl_implies` pre_g x))
+  (f:repr a pre_f post_f req_f ens_f)
+  (g:(x:a -> repr b (pre_g x) post_g (req_g x) (ens_g x)))
+: repr b
+    (pre_f `star` frame_f)
+    post_g
+    (bind_steel_steelf_req a pre_f post_f req_f ens_f pre_g req_g frame_f p)
+    (bind_steel_steelf_ens a b pre_f post_f req_f ens_f pre_g post_g ens_g frame_f p)
 = fun _ ->
   let x = frame_aux f frame_f () in
-
-  sl_implies_interp (post_f x `star` frame_f) (pre_g x);
-  sl_implies_preserves_frame (post_f x `star` frame_f) (pre_g x);
-
   (g x) ()
+
 
 polymonadic_bind (Steel, SteelF) |> SteelF = bind_steel_steelf
 
 
-let bind_steelf_steel (a:Type) (b:Type)
-  (pre_f:pre_t) (post_f:post_t a) (pre_g:a -> pre_t) (post_g:post_t b)
+(*
+ * SteelF, Steel: frame the second computation
+ *)
+
+unfold
+let bind_steelf_steel_req (a:Type)
+  (pre_f:pre_t) (post_f:post_t a)
+  (req_f:req_t pre_f) (ens_f:ens_t pre_f a post_f)  
+  (pre_g:a -> pre_t)
+  (req_g:(x:a -> req_t (pre_g x)))
   (frame_g:hprop)
-  (_:squash (forall x. post_f x `sl_implies` (pre_g x `star` frame_g)))
-  (f:repr a pre_f post_f) (g:(x:a -> repr b (pre_g x) post_g))
-: repr b pre_f (fun z -> post_g z `star` frame_g)
+  (_:squash (forall (x:a). post_f x `sl_implies` (pre_g x `star` frame_g)))
+: req_t pre_f
+= fun m0 ->
+  req_f m0 /\
+  (forall (x:a) (m1:hmem (post_f x)). ens_f m0 x m1 ==> (req_g x) m1)
+
+unfold
+let bind_steelf_steel_ens (a:Type) (b:Type)
+  (pre_f:pre_t) (post_f:post_t a)
+  (req_f:req_t pre_f) (ens_f:ens_t pre_f a post_f)  
+  (pre_g:a -> pre_t) (post_g:post_t b)
+  (ens_g:(x:a -> ens_t (pre_g x) b post_g))
+  (frame_g:hprop)
+  (_:squash (forall (x:a). post_f x `sl_implies` (pre_g x `star` frame_g)))
+: ens_t pre_f b (fun y -> post_g y `star` frame_g)
+= fun m0 y m2 ->
+  req_f m0 /\
+  (exists (x:a) (m1:hmem (post_f x)). ens_f m0 x m1 /\ (ens_g x) m1 y m2)
+
+let bind_steelf_steel (a:Type) (b:Type)
+  (pre_f:pre_t) (post_f:post_t a)
+  (req_f:req_t pre_f) (ens_f:ens_t pre_f a post_f)  
+  (pre_g:a -> pre_t) (post_g:post_t b)
+  (req_g:(x:a -> req_t (pre_g x))) (ens_g:(x:a -> ens_t (pre_g x) b post_g))
+  (frame_g:hprop)
+  (p:squash (forall (x:a). post_f x `sl_implies` (pre_g x `star` frame_g)))
+  (f:repr a pre_f post_f req_f ens_f)
+  (g:(x:a -> repr b (pre_g x) post_g (req_g x) (ens_g x)))
+: repr b
+    pre_f
+    (fun y -> post_g y `star` frame_g)
+    (bind_steelf_steel_req a pre_f post_f req_f ens_f pre_g req_g frame_g p)
+    (bind_steelf_steel_ens a b pre_f post_f req_f ens_f pre_g post_g ens_g frame_g p)
 = fun _ ->
   let x = f () in
-
-  sl_implies_interp (post_f x) (pre_g x `star` frame_g);
-  sl_implies_preserves_frame (post_f x) (pre_g x `star` frame_g);
-
   frame_aux (g x) frame_g ()
+
 
 polymonadic_bind (SteelF, Steel) |> SteelF = bind_steelf_steel
 
 
-let bind_steelf_steelf (a:Type) (b:Type)
-  (pre_f:pre_t) (post_f:post_t a) (pre_g:a -> pre_t) (post_g:post_t b)
-  (_:squash (forall x. post_f x `sl_implies` pre_g x))
-  (f:repr a pre_f post_f) (g:(x:a -> repr b (pre_g x) post_g))
-: repr b pre_f post_g
-= fun _ ->
-  let x = f () in
+(*
+ * SteelF, SteelF: no framing, use the effect bind
+ *)
 
-  sl_implies_interp (post_f x) (pre_g x);
-  sl_implies_preserves_frame (post_f x) (pre_g x);
-
-  (g x) ()
-
-polymonadic_bind (SteelF, SteelF) |> SteelF = bind_steelf_steelf
+(*
+ * PURE, Steel(F) bind
+ *)
 
 assume WP_monotonic :
   forall (a:Type) (wp:pure_wp a).
     (forall p q. (forall x. p x ==>  q x) ==>  (wp p ==>  wp q))
 
 
-(*
- * TODO: implementation of this combinator requires substitution of f and g
- *       in the comp type
- *)
+unfold
+let bind_pure_steel__req (a:Type) (wp:pure_wp a)
+  (pre:pre_t) (req:a -> req_t pre)
+: req_t pre
+= fun m -> wp (fun x -> (req x) m) /\ as_requires wp
+
+unfold
+let bind_pure_steel__ens (a:Type) (b:Type)
+  (wp:pure_wp a)
+  (pre:pre_t) (post:post_t b) (ens:a -> ens_t pre b post)
+: ens_t pre b post
+= fun m0 r m1 -> as_requires wp /\ (exists (x:a). as_ensures wp x /\ (ens x) m0 r m1)
+
 let bind_pure_steel_ (a:Type) (b:Type)
-  (wp:pure_wp a) (pre_g:a -> pre_t) (post_g:a -> post_t b)
-  (_:squash (wp (fun _ -> True)))
-  (f:unit -> PURE a wp) (g:(x:a -> repr b (pre_g x) (post_g x)))
-: repr b (pre_g (f ())) (post_g (f ()))
+  (wp:pure_wp a)
+  (pre:pre_t) (post:post_t b) (req:a -> req_t pre) (ens:a -> ens_t pre b post)
+  (f:unit -> PURE a wp) (g:(x:a -> repr b pre post (req x) (ens x)))
+: repr b
+    pre
+    post
+    (bind_pure_steel__req a wp pre req)
+    (bind_pure_steel__ens a b wp pre post ens)
 = fun _ ->
   let x = f () in
   (g x) ()
@@ -278,41 +447,14 @@ polymonadic_bind (PURE, SteelF) |> SteelF = bind_pure_steel_
 
 polymonadic_bind (PURE, Steel) |> Steel = bind_pure_steel_
 
-// let bind_pure_steel (a:Type) (b:Type)
-//   (pre_f:pre_t) (post_f:post_t a) (wp:a -> pure_wp b)
-//   (frame_f:hprop) (post_g:post_t b)
-//   (_:squash (forall x. wp x (fun _ -> True)))
-//   (f:repr a pre_f post_f) (g:(x:a -> unit -> PURE b (wp x)))
-//   (_:squash (forall x. (post_f x `star` frame_f) `sl_implies` (post_g (g x ()))))
-// : repr b (pre_f `star` frame_f) post_g
-// = fun _ ->
-//   let x = (frame_aux f frame_f) () in
-//   let y = (g x) () in
 
-//   sl_implies_interp (post_f x `star` frame_f) (post_g y);
-//   sl_implies_preserves_frame_right (post_f x `star` frame_f) (post_g y);
-
-//   y
-
-// // TODO:
-// // polymonadic_bind (Steel, PURE) |> SteelF = bind_pure_steel
-
-
-// let bind_pure_steelf (a:Type) (b:Type)
-//   (pre_f:pre_t) (post_f:post_t a) (wp:a -> pure_wp b)
-//   (post_g:post_t b)
-//   (_:squash (forall x. wp x (fun _ -> True)))
-//   (f:repr a pre_f post_f) (g:(x:a -> unit -> PURE b (wp x)))
-//   (_:squash (forall x. post_f x `sl_implies` (post_g (g x ()))))
-// : repr b pre_f post_g
-// = fun _ ->
-//   let x = f () in
-//   let y = (g x) () in
-
-//   sl_implies_interp (post_f x) (post_g y);
-//   sl_implies_preserves_frame_right (post_f x) (post_g y);
-  
-//   y
-
-// // TODO:
-// // polymonadic_bind (SteelF, PURE) |> SteelF = bind_pure_steelf
+(*
+ * No Steel(F), PURE bind
+ *
+ * Use the steel_ret function below to return the PURE computation
+ *
+ * Note it is in SteelF (i.e. framed already)
+ *)
+let steel_ret (a:Type) (x:a) (#p:a -> hprop u#1)
+: SteelF a (p x) p (fun _ -> True) (fun _ r _ -> r == x)
+= SteelF?.reflect (fun _ -> x)
